@prefix : <https://blue-room-innovation.github.io/dcasr-ontology/codelists/v0.1/discharge-means-code.ttl#> .
@prefix skos: <http://www.w3.org/2004/02/skos/core#> .
@prefix owl: <http://www.w3.org/2002/07/owl#> .
@prefix xsd: <http://www.w3.org/2001/XMLSchema#> .
@prefix rdfs: <http://www.w3.org/2000/01/rdf-schema#> .

@base <https://blue-room-innovation.github.io/dcasr-ontology/codelists/v0.1/discharge-means-code.ttl> .

<https://blue-room-innovation.github.io/dcasr-ontology/codelists/v0.1/discharge-means-code.ttl> a owl:Ontology ;
    rdfs:label "Discharge Means Code List"@en ;
    owl:versionInfo "0.1" ;
    rdfs:comment "A SKOS vocabulary that specifies the means or method of discharge for a particular residue or waste material under MARPOL regulations."@en .

#################################################################
#    Concept Scheme
#################################################################

:DischargeMeansCodeScheme a skos:ConceptScheme ;
    skos:prefLabel "Discharge Means Code"@en ;
    skos:definition "A code that specifies the means or method of discharge for a particular residue or waste material."@en ;
    rdfs:comment "Defines the possible discharge methods under MARPOL waste handling processes."@en .

#################################################################
#    Concepts
#################################################################

:ZTE a skos:Concept ;
    skos:inScheme :DischargeMeansCodeScheme ;
    skos:prefLabel "ZTE"@en ;
    skos:definition "Discharge to a port reception facility."@en .

:ZTD a skos:Concept ;
    skos:inScheme :DischargeMeansCodeScheme ;
    skos:prefLabel "ZTD"@en ;
    skos:definition "Discharge to a designated waste treatment system."@en .

:ZTC a skos:Concept ;
    skos:inScheme :DischargeMeansCodeScheme ;
    skos:prefLabel "ZTC"@en ;
    skos:definition "Direct discharge to sea (per MARPOL regulations)."@en .

:ZTB a skos:Concept ;
    skos:inScheme :DischargeMeansCodeScheme ;
    skos:prefLabel "ZTB"@en ;
    skos:definition "Discharge to a designated waste collection area."@en .

#################################################################
#    Ontology linkage
#################################################################

:DischargeMeansCodeScheme skos:note "Linked to the property :dischargeMeans in the Digital MARPOL Waste Passport ontology, constraining allowed values to this controlled vocabulary."@en .
