@prefix : <https://blue-room-innovation.github.io/dcasr-ontology/codelists/v0.1/residue-type-code.ttl#> .
@prefix skos: <http://www.w3.org/2004/02/skos/core#> .
@prefix owl: <http://www.w3.org/2002/07/owl#> .
@prefix dcterms: <http://purl.org/dc/terms/> .
@prefix xsd: <http://www.w3.org/2001/XMLSchema#> .
@prefix rdfs: <http://www.w3.org/2000/01/rdf-schema#> .

@base <https://blue-room-innovation.github.io/dcasr-ontology/codelists/v0.1/residue-type-code.ttl> .

<https://blue-room-innovation.github.io/dcasr-ontology/codelists/v0.1/residue-type-code.ttl> a owl:Ontology ;
    rdfs:label "Residue Type Code List"@en ;
    owl:versionInfo "0.1" ;
    rdfs:comment "A SKOS vocabulary that specifies the type of residue (waste material) generated by the ship, as defined by a local codelist adhering to MARPOL standards. It supports the classification of waste types ensuring that materials are correctly identified and handled according to regulatory requirements."@en ;
    dcterms:creator "CircularPass Ontology Team" ;
    dcterms:source "Digital MARPOL Waste Passport Code Table" ;
    dcterms:issued "2025-11-10"^^xsd:date .

#################################################################
#    Concept Scheme
#################################################################

:ResidueTypeCodeScheme a skos:ConceptScheme ;
    skos:prefLabel "Residue Type Code"@en ;
    skos:definition "A code that specifies the type of residue (waste material) generated by the ship, as defined by MARPOL standards."@en ;
    rdfs:comment "Defines the main waste types under MARPOL Annexes, such as hazardous, non-hazardous, sludge, and wastewater residues."@en .

#################################################################
#    Concepts
#################################################################

:ZTH a skos:Concept ;
    skos:inScheme :ResidueTypeCodeScheme ;
    skos:prefLabel "ZTH"@en ;
    skos:definition "Hazardous liquid waste (as per MARPOL Annex II)."@en .

:ZTE a skos:Concept ;
    skos:inScheme :ResidueTypeCodeScheme ;
    skos:prefLabel "ZTE"@en ;
    skos:definition "Non-hazardous solid waste."@en .

:ZTR a skos:Concept ;
    skos:inScheme :ResidueTypeCodeScheme ;
    skos:prefLabel "ZTR"@en ;
    skos:definition "Sludge waste."@en .

:ZTW a skos:Concept ;
    skos:inScheme :ResidueTypeCodeScheme ;
    skos:prefLabel "ZTW"@en ;
    skos:definition "Wastewater (from ship operations)."@en .

#################################################################
#    Ontology linkage
#################################################################

:ResidueTypeCodeScheme skos:note "Linked to the property :typeCode in the Digital MARPOL Waste Passport ontology, constraining allowed values to this controlled vocabulary."@en .
